\section{Proof of $\vec{a}\times(\vec{b}\times\vec{c}) = (\vec{c}\cdot\vec{a})\vec{b} - (\vec{b}\cdot\vec{a})\vec{c}$}

Let $\vec{a}$, $\vec{b}$, $\vec{c}$ be three dimentional vectors where

\[
    \vec{a} = \begin{vmatrix}
        p \\
        q \\
        r 
    \end{vmatrix} \;
    \vec{b} = \begin{vmatrix}
        s \\
        t \\
        u
    \end{vmatrix} \;
    \vec{c} = \begin{vmatrix}
        x \\
        y \\
        z
    \end{vmatrix}
\]

hence

\[
    \vec{b}\times\vec{c} = \det\begin{vmatrix}
        \vec{i} & \vec{j} & \vec{k} \\
        s & t & u \\
        x & y & z
    \end{vmatrix} = \vec{i}(tz-uy) + \vec{j}(ux-sz) + \vec{k}(sy-tx) = \begin{vmatrix}
        tz - uy \\
        ux - sz \\
        sy - tx
    \end{vmatrix} = \begin{vmatrix}
        \alpha \\
        \beta \\
        \gamma
    \end{vmatrix}
\]

Thus

\[
    \vec{a}\times(\vec{b}\times\vec{c}) = \vec{a}\times\begin{vmatrix}
        \alpha \\
        \beta \\
        \gamma
    \end{vmatrix} = \det\begin{vmatrix}
        \vec{i} & \vec{j} & \vec{k} \\
        p & q & r \\
        \alpha & \beta & \gamma
    \end{vmatrix} = \vec{i}(q\gamma - r\beta) + \vec{j}(r\alpha - p\gamma) + \vec{k}(p\beta - q\alpha) =
    \begin{vmatrix}
        q\gamma - r\beta \\
        r\alpha - p\gamma \\
        p\beta - q\alpha
    \end{vmatrix}
\]

Now working on the right hand side of the equation,

\[
\begin{aligned}
    \vec{a}\cdot\vec{b} & = ps + qt + ru \\
    \vec{a}\cdot\vec{c} & = px + qy + rz
\end{aligned}
\]

\[
    (\vec{a}\cdot\vec{c})\vec{b} - (\vec{a}\cdot\vec{b})\vec{c} = (px + qy + rz)\begin{vmatrix}
        s \\
        t \\
        u
    \end{vmatrix} - (ps + qt + ru)\begin{vmatrix}
        x \\
        y \\
        z
    \end{vmatrix} = \begin{vmatrix}
        psx + qsy + rsz \\
        ptx + qty + rtz \\
        pux + quy + ruz
    \end{vmatrix} - \begin{vmatrix}
        psx + qtx + rux \\
        psy + qty + ruy \\
        psz + qtz + ruz
    \end{vmatrix}
\]

\[
    = \begin{vmatrix}      
        qsy + rsz - qtx - rux \\
        ptx + rtz - psy - ruy \\
        pux + quy - psz - qtz
    \end{vmatrix} = \begin{vmatrix}
        q (sy - tx) - r (ru - sz) \\
        r (tz - uy) - p (sy - tx)  \\
        p (ux - sz) - q (tz - uy)
    \end{vmatrix} = \begin{vmatrix}
        q\gamma - r\beta \\
        r\alpha - p\gamma \\
        p\beta - q\alpha
    \end{vmatrix} = \vec{a}\times(\vec{b}\times\vec{c})
\]