\section{Proof of $\vec{a}\times\vec{b} = \lvert\vec{a}\rvert\lvert\vec{b}\rvert\lvert\sin\phi\rvert$}

Using the previously proven Langrange equation, the eqaution above is easily proven.

\[
\begin{aligned}
    \lvert\vec{a}\times\vec{b}\rvert^2 & = \lvert\vec{a}\rvert^2\lvert\vec{b}\rvert^2- (\vec{a}\cdot\vec{b})^2 \\
    \vec{a}\cdot\vec{b} & = \lvert\vec{a}\rvert\lvert\vec{b}\rvert\cos\phi \\
    \vec{a}\cdot\vec{b}^2 & = \lvert\vec{a}\rvert^2\lvert\vec{b}\rvert^2\cos^2\phi \\
    \lvert\vec{a}\times\vec{b}\rvert^2 & = \lvert\vec{a}\rvert^2\lvert\vec{b}\rvert^2 - 
        \lvert\vec{a}\rvert^2\lvert\vec{b}\rvert^2\cos^2\phi\\
    \lvert\vec{a}\times\vec{b}\rvert^2 & = \lvert\vec{a}\rvert^2\lvert\vec{b}\rvert^2(1-\cos^2\phi) \\
    \lvert\vec{a}\times\vec{b}\rvert^2 & = \lvert\vec{a}\rvert^2\lvert\vec{b}\rvert^2(\sin^2\phi) \\
    \lvert\vec{a}\times\vec{b}\rvert & = \lvert\vec{a}\rvert\lvert\vec{b}\rvert \lvert\sin\phi\rvert \\
\end{aligned}
\]